examples/arm6/lemmasScript.sml
@@ -189,48 +189,68 @@ val MEMREAD_ALIGNED = store_thm("MEMREAD_ALIGNED",
 
 (* -------------------------------------------------------- *)
 
+val REGISTER_RANGES = save_thm("REGISTER_RANGES",
+  let fun conj (a,b) = CONJ a b in
+   foldl conj (DECIDE ``14 < 16``)
+     (map REDUCE_RULE [SPECL [`19`,`16`] BITSwLT_THM,
+                       SPECL [`15`,`12`] BITSwLT_THM,
+                       SPECL [`11`,`8`] BITSwLT_THM,
+                       SPECL [`3`,`0`] BITSwLT_THM])
+  end
+);
+
+(* -------------------------------------------------------- *)
+
 val PC_WRITE_MODE_FREE = store_thm("PC_WRITE_MODE_FREE",
   `!r m p. REG_WRITE r m 15 p = REG_WRITE r usr 15 p`,
-  Cases THEN RW_TAC std_ss [REG_WRITE_def]
+  RW_TAC bool_ss [mode_num2register_def,REG_WRITE_def]
 );
-
+ 
 val PC_READ_MODE_FREE = store_thm("PC_READ_MODE_FREE",
   `!r m p. REG_READ6 r m 15 = REG_READ6 r usr 15`,
-  RW_TAC std_ss [REG_READ6_def]
+  RW_TAC bool_ss [REG_READ6_def]
 );
-
+ 
 val REG_WRITE_READ_PC = store_thm("REG_WRITE_READ_PC",
   `!r m p. REG_READ6 (REG_WRITE r m 15 p) usr 15 = p`,
-  Cases THEN RW_TAC std_ss [REG_READ6_def,FETCH_PC_def,REG_WRITE_def,SUBST_def]
+  RW_TAC bool_ss [REG_READ6_def,FETCH_PC_def,REG_WRITE_def,SUBST_def,
+                  mode_num2register_def,r15,register2num_thm]
 );
-
+ 
 val REG_WRITE_WRITE_PC = store_thm("REG_WRITE_WRITE_PC",
   `!r m1 m2 p1 p2. REG_WRITE (REG_WRITE r m1 15 p1) m2 15 p2 = REG_WRITE r m2 15 p2`,
-  Cases THEN RW_TAC std_ss [REG_WRITE_def,SUBST_EQ]
+  RW_TAC bool_ss [REG_WRITE_def,SUBST_EQ,mode_num2register_def]
+);
+ 
+val NOT_PC_THM = store_thm("NOT_PC_THM",
+  `!m1 m2 n. n < 16 /\ ~(n = 15) ==> ~(mode_num2register m1 n = mode_num2register m2 15)`,
+  RW_TAC bool_ss [mode_num2register_def,USER_def]
+    THEN FULL_SIMP_TAC arith_ss [mode_case_def,register2num_11,num2register_11]
+    THEN Cases_on `m1`
+    THEN FULL_SIMP_TAC arith_ss [mode_case_def,num2register_11]
 );
 
 val REG_WRITE_COMMUTES = store_thm("REG_WRITE_COMMUTES",
-  `!r m1 m2 n d p. ~(n = 15) ==> (REG_WRITE (REG_WRITE r m1 15 p) m2 n d = REG_WRITE (REG_WRITE r m2 n d) m1 15 p)`,
-  REPEAT STRIP_TAC
-    THEN ONCE_REWRITE_TAC [PC_WRITE_MODE_FREE]
-    THEN Cases_on `r`
-    THEN Cases_on `m2`
-    THEN RW_TAC std_ss [REG_WRITE_def,SUBST_NE_COMMUTES,USER_def]
+  `!r m1 m2 n d p.
+      n < 16 /\ ~(n = 15) ==>
+      (REG_WRITE (REG_WRITE r m1 15 p) m2 n d =
+       REG_WRITE (REG_WRITE r m2 n d) m1 15 p)`,
+  RW_TAC bool_ss [REG_WRITE_def,SUBST_NE_COMMUTES,NOT_PC_THM]
 );
-
+ 
 val REG_WRITE_READ_R14 = store_thm("REG_WRITE_READ_R14",
   `!r m m2 d x. REG_READ6 (REG_WRITE (REG_WRITE r m 14 d) m2 15 x) m 14 = d`,
   REPEAT STRIP_TAC
     THEN ONCE_REWRITE_TAC [PC_WRITE_MODE_FREE]
-    THEN SIMP_TAC arith_ss [GSYM REG_WRITE_COMMUTES]
-    THEN Cases_on `r`
+    THEN RW_TAC arith_ss [mode_num2register_def,REG_READ6_def,REG_READ_def,
+                          REG_WRITE_def,SUBST_NE_COMMUTES,SUBST_def,USER_def]
     THEN Cases_on `m`
-    THEN RW_TAC arith_ss [REG_READ6_def,REG_READ_def,REG_WRITE_def,SUBST_def,USER_def]
+    THEN FULL_SIMP_TAC arith_ss [mode_case_def,mode_distinct,GSYM mode_distinct,num2register_11,register2num_11]
 );
-
+ 
 val REG_WRITE_WRITE_R14 = store_thm("REG_WRITE_WRITE_R14",
   `!r m d1 d2. REG_WRITE (REG_WRITE r m 14 d1) m 14 d2 = REG_WRITE r m 14 d2`,
-  Cases THEN Cases THEN RW_TAC std_ss [REG_WRITE_def,SUBST_EQ,USER_def]
+  RW_TAC bool_ss [REG_WRITE_def,SUBST_EQ,USER_def,mode_num2register_def]
 );
 
 (* -------------------------------------------------------- *)
@@ -275,39 +295,44 @@ val SUBST_EQ2 = store_thm("SUBST_EQ2",
   `!m a. SUBST m (a,m a) = m`,
   STRIP_TAC THEN SIMP_TAC bool_ss [FUN_EQ_THM,SUBST_def]
 );
-
+ 
 val SUB8_INV = store_thm("SUB8_INV",
   `!r. SUB8_PC (ADD8_PC r) = r`,
-  Cases THEN RW_TAC std_ss [ADD_SUBw,SUB8_PC_def,ADD8_PC_def,SUBST_EQ,SUBST_EQ2,SUBST_def]
+  RW_TAC bool_ss [ADD_SUBw,SUB8_PC_def,ADD8_PC_def,SUBST_EQ,SUBST_EQ2,SUBST_def]
 );
-
+ 
 val FETCH_SUB8 = store_thm("FETCH_SUB8",
   `!r.  FETCH_PC (SUB8_PC r) = REG_READ6 r usr 15 - w32 8`,
-  Cases THEN RW_TAC std_ss [FETCH_PC_def,REG_READ6_def,SUB8_PC_def,SUBST_def]
+  RW_TAC bool_ss [FETCH_PC_def,REG_READ6_def,SUB8_PC_def,SUBST_def]
 );
+ 
+val mode_num2register_15 = GEN_ALL (SIMP_RULE arith_ss [SYM r15] (SPECL [`m`,`15`] mode_num2register_def));
 
 val REG_READ_SUB8_PC = store_thm("REG_READ_SUB8_PC",
-  `!r m n. REG_READ (SUB8_PC r) m n = REG_READ6 r m n`,
-  Cases THEN RW_TAC std_ss [SUBST_def,REG_READ_def,REG_READ6_def,SUB8_PC_def,FETCH_PC_def,
-                            ONCE_REWRITE_RULE [ADD_SUB_SYM] ADD_SUBw]
+  `!r m n. n < 16 ==> (REG_READ (SUB8_PC r) m n = REG_READ6 r m n)`,
+  RW_TAC bool_ss [REG_READ_def,REG_READ6_def,SUB8_PC_def,FETCH_PC_def]
+    THEN ASM_SIMP_TAC arith_ss [SUBST_def,ONCE_REWRITE_RULE [ADD_SUB_SYM] ADD_SUBw]
+    THEN SUBST_TAC [SYM (SPEC `m` mode_num2register_15)]
+    THEN ASM_SIMP_TAC bool_ss [NOT_PC_THM]
 );
-
+ 
 val NOOP_REG = store_thm("NOOP_REG",
   `!r m.  INC_PC (SUB8_PC r) = SUB8_PC (REG_WRITE r m 15 (REG_READ6 r usr 15 + w32 4))`,
-  Cases THEN RW_TAC std_ss [INC_PC_def,SUB8_PC_def,REG_WRITE_def,REG_READ6_def,
-                            FETCH_PC_def,SUBST_def,SUBST_EQ,ADD_SUB_SYM]
+  RW_TAC bool_ss [INC_PC_def,SUB8_PC_def,REG_WRITE_def,REG_READ6_def,mode_num2register_def,
+                  SYM r15,FETCH_PC_def,SUBST_def,SUBST_EQ,ADD_SUB_SYM]
 );
-
+ 
 val OP_REG_LEM = store_thm("OP_REG_LEM",
   `!r m d. REG_WRITE (SUB8_PC r) m 15 d = SUB8_PC (REG_WRITE r m 15 (d + w32 4 + w32 4))`,
-  ONCE_REWRITE_TAC [PC_WRITE_MODE_FREE]
-    THEN Cases
-    THEN RW_TAC std_ss [REG_WRITE_def,SUB8_PC_def,SUBST_def,SUBST_EQ,ADD4_ADD4_SUB8_THM]
+  RW_TAC bool_ss [mode_num2register_def,SYM r15,REG_WRITE_def,
+                  SUB8_PC_def,SUBST_def,SUBST_EQ,ADD4_ADD4_SUB8_THM]
 );
-
+ 
 val INC_REG_LEM = store_thm("INC_REG_LEM",
-  `!r m n d. ~(n = 15) ==> (REG_WRITE (SUB8_PC r) m n d = SUB8_PC (REG_WRITE r m n d))`,
-  Cases THEN Cases THEN RW_TAC std_ss [SUBST_NE_COMMUTES,FETCH_PC_def,SUB8_PC_def,REG_WRITE_def,SUBST_def,USER_def]
+  `!r m n d. n < 16 /\ ~(n = 15) ==> (REG_WRITE (SUB8_PC r) m n d = SUB8_PC (REG_WRITE r m n d))`,
+  RW_TAC bool_ss [FETCH_PC_def,SUB8_PC_def,REG_WRITE_def]
+    THEN SUBST_TAC [SYM (SPEC `m` mode_num2register_15)]
+    THEN ASM_SIMP_TAC bool_ss [SUBST_def,SUBST_NE_COMMUTES,NOT_PC_THM]
 );
 
 val OP_REG = store_thm("OP_REG",
@@ -317,7 +342,7 @@ val OP_REG = store_thm("OP_REG",
     THEN SIMP_TAC std_ss [ONCE_REWRITE_RULE [PC_WRITE_MODE_FREE] NOOP_REG,
                           REG_WRITE_WRITE_PC,OP_REG_LEM]
 );
-
+ 
 val INC_WB_REG = store_thm("INC_WB_REG",
   `!r m d. INC_PC (SUB8_PC (REG_WRITE r m 15 d)) = SUB8_PC (REG_WRITE r m 15 (d + w32 4))`,
   ONCE_REWRITE_TAC [PC_WRITE_MODE_FREE]
@@ -326,40 +351,39 @@ val INC_WB_REG = store_thm("INC_WB_REG",
 );
  
 val INC_PC_READ = store_thm("INC_PC_READ",
-  `!r m n. REG_READ (INC_PC (SUB8_PC r)) m n =
-             REG_READ6 (REG_WRITE r m 15 (REG_READ6 r usr 15 + w32 4)) m n`,
+  `!r m n. n < 16 ==> (REG_READ (INC_PC (SUB8_PC r)) m n =
+             REG_READ6 (REG_WRITE r m 15 (REG_READ6 r usr 15 + w32 4)) m n)`,
   ONCE_REWRITE_TAC [PC_WRITE_MODE_FREE]
-    THEN SIMP_TAC std_ss [ONCE_REWRITE_RULE [PC_WRITE_MODE_FREE] NOOP_REG,REG_READ_SUB8_PC]
+    THEN SIMP_TAC bool_ss [ONCE_REWRITE_RULE [PC_WRITE_MODE_FREE] NOOP_REG,REG_READ_SUB8_PC]
 );
-
+ 
 val OP_INC_REG = store_thm("OP_INC_REG",
-  `!r m n. ~(n = 15) ==> (REG_WRITE (INC_PC (SUB8_PC r)) m n d =
-       SUB8_PC (
-         (REG_WRITE (REG_WRITE r m n d) m 15 (REG_READ6 r usr 15 + w32 4))))`,
+  `!r m n. n < 16 /\ ~(n = 15) ==> (REG_WRITE (INC_PC (SUB8_PC r)) m n d =
+       SUB8_PC (REG_WRITE (REG_WRITE r m n d) m 15 (REG_READ6 r usr 15 + w32 4)))`,
   ONCE_REWRITE_TAC [PC_WRITE_MODE_FREE]
-    THEN RW_TAC std_ss [ONCE_REWRITE_RULE [PC_WRITE_MODE_FREE] NOOP_REG,INC_REG_LEM,REG_WRITE_COMMUTES]
+    THEN SIMP_TAC bool_ss [ONCE_REWRITE_RULE [PC_WRITE_MODE_FREE] NOOP_REG,INC_REG_LEM,REG_WRITE_COMMUTES]
 );
 
 val OP_REG2 = store_thm("OP_REG2",
-  `!r m m2 n x y.  REG_WRITE (REG_WRITE (INC_PC (SUB8_PC r)) m n x) m2 15 y =
-                 SUB8_PC (REG_WRITE (REG_WRITE r m n x) m2 15 (y + w32 4 + w32 4))`,
+  `!r m m2 n x y.  n < 16 ==>
+         (REG_WRITE (REG_WRITE (INC_PC (SUB8_PC r)) m n x) m2 15 y =
+          SUB8_PC (REG_WRITE (REG_WRITE r m n x) m2 15 (y + w32 4 + w32 4)))`,
   ONCE_REWRITE_TAC [PC_WRITE_MODE_FREE]
     THEN REPEAT STRIP_TAC
     THEN Cases_on `n = 15`
     THENL [
-      ASM_SIMP_TAC std_ss [REG_WRITE_WRITE_PC] THEN REWRITE_TAC [OP_REG],
-      ASM_SIMP_TAC std_ss [ONCE_REWRITE_RULE [PC_WRITE_MODE_FREE] NOOP_REG,REG_WRITE_COMMUTES,
-                           REG_WRITE_WRITE_PC,INC_REG_LEM,OP_REG_LEM]
+      ASM_SIMP_TAC bool_ss [REG_WRITE_WRITE_PC] THEN REWRITE_TAC [OP_REG],
+      ASM_SIMP_TAC bool_ss [ONCE_REWRITE_RULE [PC_WRITE_MODE_FREE] NOOP_REG,REG_WRITE_COMMUTES,                           REG_WRITE_WRITE_PC,INC_REG_LEM,OP_REG_LEM]
     ]
 );
  
 val OP_INC_REG2 = store_thm("OP_INC_REG2",
-  `!r m m2 m3 n n2 x y.  ~(n = 15) /\ ~(n2 = 15) ==>
+  `!r m m2 m3 n n2 x y.  n < 16 /\ n2 < 16 /\ ~(n = 15) /\ ~(n2 = 15) ==>
     (REG_WRITE (REG_WRITE (INC_PC (SUB8_PC r)) m n x) m2 n2 y =
      SUB8_PC (REG_WRITE (REG_WRITE (REG_WRITE r m n x) m2 n2 y)
                         m3 15 (REG_READ6 r usr 15 + w32 4)))`,
   ONCE_REWRITE_TAC [PC_WRITE_MODE_FREE]
-    THEN RW_TAC std_ss [ONCE_REWRITE_RULE [PC_WRITE_MODE_FREE] NOOP_REG,INC_REG_LEM,REG_WRITE_COMMUTES]
+    THEN SIMP_TAC bool_ss [ONCE_REWRITE_RULE [PC_WRITE_MODE_FREE] NOOP_REG,INC_REG_LEM,REG_WRITE_COMMUTES]
 );
  
 val LINK_REG = store_thm("LINK_REG",
@@ -368,7 +392,7 @@ val LINK_REG = store_thm("LINK_REG",
   ONCE_REWRITE_TAC [PC_WRITE_MODE_FREE]
     THEN SIMP_TAC arith_ss [OP_REG_LEM,INC_REG_LEM]
 );
- 
+
 val BRANCH_REG = store_thm("BRANCH_REG",
   `!r m y.  REG_WRITE (SUB8_PC r) usr 15 y =
                  SUB8_PC (REG_WRITE r m 15 (y + w32 4 + w32 4))`,
